\section{Smith-Diagramm}

\subsection{Allgemein}
\begin{center}
    \begin{align*}
        \Aboxed{r(z) & = r_A \cdot e^{-j2\beta z}}
    \end{align*}
    \input{Figures/Smithdiagramm_Smithchart.tex}
\end{center}
\begin{align*}
    \underline{z}_n & = \frac{\underline{Z}_n}{Z_L}                                                                                                                   \\
    \underline{r}_n & = \frac{\underline{Z}_n-Z_L}{\underline{Z}_n+Z_L}= \frac{\underline{z}_n-1}{\underline{z}_n+1}    = \frac{1-\underline{y}_n}{1+\underline{y}_n} \\
    m               & = \frac{1-|\underline{r}|}{1+|\underline{r}|}
\end{align*}
